DataflowRewriter/ExprHigh.lean
@@ -6,6 +6,7 @@ Authors: Yann Herklotz
 
 import Lean
 import DataflowRewriter.ExprLow
+import Qq
 
 namespace DataflowRewriter
 
@@ -258,10 +259,10 @@ def rename [FreshIdent Ident]
 
 end ExprHigh
 
-def updatePortMappingInput (s : Std.HashMap String (PortMapping String × String))
+def updatePortMappingInput {α} [Inhabited α] (s : Std.HashMap String (PortMapping String × α))
   (inCluster : Bool)
   (inPort : InternalPort String)
-  : Bool → InternalPort String → Std.HashMap String (PortMapping String × String)
+  : Bool → InternalPort String → Std.HashMap String (PortMapping String × α)
 | _, co@⟨.top, n⟩ =>
   match (inCluster, inPort) with
   | (true, ci@⟨.internal x, y⟩) =>
@@ -276,10 +277,10 @@ def updatePortMappingInput (s : Std.HashMap String (PortMapping String × String
   s.insert i ({a with input := a.input.cons ⟨.top, x⟩ c}, b)
 | true, ⟨.internal _, _⟩ => s
 
-def updatePortMappingOutput (s : Std.HashMap String (PortMapping String × String))
+def updatePortMappingOutput {α} [Inhabited α] (s : Std.HashMap String (PortMapping String × α))
   (inCluster : Bool)
   (inPort : InternalPort String)
-  : Bool → InternalPort String → Std.HashMap String (PortMapping String × String)
+  : Bool → InternalPort String → Std.HashMap String (PortMapping String × α)
 | _, co@⟨.top, n⟩ =>
   match (inCluster, inPort) with
   | (true, ci@⟨.internal x, y⟩) =>
@@ -304,6 +305,11 @@ structure InstMaps where
   instMap : Std.HashMap String (InstIdent String × Bool)
   instTypeMap : Std.HashMap String (PortMapping String × String)
 
+open Lean Qq in
+structure InstMaps' where
+  instMap : Std.HashMap String (InstIdent String × Bool)
+  instTypeMap : Std.HashMap String (PortMapping String × Q(String))
+
 def updateNodeMaps (maps : InstMaps) (inst typ : String) (cluster : Bool := false) : Except String InstMaps := do
   let mut instMap := maps.instMap
   let mut instTypeMap := maps.instTypeMap
@@ -314,6 +320,21 @@ def updateNodeMaps (maps : InstMaps) (inst typ : String) (cluster : Bool := fals
     instMap := map'
     -- IO "modules" are not added to the instTypeMap.
     unless typ == "io" do instTypeMap := instTypeMap.insert inst (∅, typ)
+  else
+    throw s!"Multiple references to {inst} found"
+  return ⟨instMap, instTypeMap⟩
+
+open Lean Qq in
+def updateNodeMaps' (maps : InstMaps') (inst : String) (typ : Q(String)) (cluster : Bool := false) : Except String InstMaps' := do
+  let mut instMap := maps.instMap
+  let mut instTypeMap := maps.instTypeMap
+  let mut modInst : InstIdent String := .top
+  unless typ == toExpr "io" do modInst := .internal inst
+  let (b, map') := instMap.containsThenInsertIfNew inst (modInst, cluster)
+  if !b then
+    instMap := map'
+    -- IO "modules" are not added to the instTypeMap.
+    unless typ == toExpr "io" do instTypeMap := instTypeMap.insert inst (∅, typ)
   else
     throw s!"Multiple references to {inst} found"
   return ⟨instMap, instTypeMap⟩
@@ -334,6 +355,43 @@ instance : ToString ConnError where
 def updateConnMaps (maps : InstMaps) (conns : List (Connection String))
     (outInst inInst : String) (outP inP : Option String)
     : Except ConnError (InstMaps × List (Connection String)) := do
+  let mut out := outP
+  let mut inp := inP
+  let some aInst := maps.instMap[outInst]? | throw (.outInstError "Instance has not been declared")
+  let some bInst := maps.instMap[inInst]? | throw (.inInstError "Instance has not been declared")
+  if aInst.fst = .top && bInst.fst = .top then
+    throw <| .outInstError "Both the input and output are IO ports"
+  -- If no port name is provided and the port is a top-level port, then use
+  -- the instance name as the port name.
+  if out.isNone && aInst.fst.isTop then out := some outInst
+  if inp.isNone && bInst.fst.isTop then inp := some inInst
+  let some out' := out | throw <| .portError s!"No output found for: {aInst}"
+  let some inp' := inp | throw <| .portError s!"No input found for: {bInst}"
+  let some outPort := parseInternalPort out'
+    | throw <| .portError "Output port format incorrect"
+  let some inPort := parseInternalPort inp'
+    | throw <| .portError "Input port format incorrect"
+  -- If the instance is a cluster do not modify the name, otherwise as the
+  -- instance as a prefix.
+  let outPort' := if aInst.snd then outPort else ⟨aInst.fst, outPort.name⟩
+  let inPort' := if bInst.snd then inPort else ⟨bInst.fst, inPort.name⟩
+  -- If one of the end points is an external port then do not add a
+  -- connection into the graph.
+  let mut conns := conns
+  let mut instTypeMap := maps.instTypeMap
+  unless aInst.fst = .top || bInst.fst = .top do
+    conns := ⟨ outPort', inPort' ⟩ :: conns
+    instTypeMap := updatePortMappingOutput instTypeMap bInst.snd inPort' aInst.snd outPort'
+    instTypeMap := updatePortMappingInput instTypeMap aInst.snd outPort' bInst.snd inPort'
+  if aInst.fst = .top then
+    instTypeMap := updatePortMappingOutput instTypeMap bInst.snd inPort' aInst.snd outPort'
+  if bInst.fst = .top then
+    instTypeMap := updatePortMappingInput instTypeMap aInst.snd outPort' bInst.snd inPort'
+  return (⟨maps.instMap, instTypeMap⟩, conns)
+
+def updateConnMaps' (maps : InstMaps') (conns : List (Connection String))
+    (outInst inInst : String) (outP inP : Option String)
+    : Except ConnError (InstMaps' × List (Connection String)) := do
   let mut out := outP
   let mut inp := inP
   let some aInst := maps.instMap[outInst]? | throw (.outInstError "Instance has not been declared")
